theories/ordinals/MoreAck/fol_Examples.v
@@ -1,5 +1,5 @@
 From Coq Require Import Arith Lists.List.
-Require Import fol Languages.
+Require Import fol folProp Languages.
 Require Import primRec.
 
 (* begin snippet arityTest *)
@@ -28,58 +28,108 @@ Notation Tcons := (Tcons LNN _).
 Notation Tnil := (Tnil LNN). 
 Notation var := (var LNN).
 Notation apply := (apply LNN). 
-Notation forallNN := (forallH LNN).
-Notation atomicNN := (atomic LNN). 
-Notation impNN := (impH LNN).
-Notation notNN := (notH LNN).
+Notation forallH := (forallH LNN).
+Notation atomic := (atomic LNN). 
+Notation inpH := (impH LNN).
+Notation notH := (notH LNN).
 Notation equal t1 t2 := (equal LNN t1 t2).
 
-Notation orNN := (orH LNN).
-Notation andNN := (andH LNN).
-Notation iffNN := (iffH LNN).
-Notation existNN := (existH LNN).
+Notation orH := (orH LNN).
+Notation andH := (andH LNN).
+Notation iffH := (iffH LNN).
+Notation existH := (existH LNN).
 
 
-Notation plusNN t1 t2:= (apply Plus (Tcons t1 (Tcons t2 Tnil))).
-Notation ltNN t1 t2 := (atomicNN LT (Tcons t1 (Tcons t2 Tnil))). 
-Notation zeroNN := (apply Zero Tnil).
-Notation succNN t := (apply Succ (Tcons t Tnil)).
+Notation plusH t1 t2:= (apply Plus (Tcons t1 (Tcons t2 Tnil))).
+Notation timesH t1 t2:= (apply Times (Tcons t1 (Tcons t2 Tnil))).
+Notation ltH t1 t2 := (atomic LT (Tcons t1 (Tcons t2 Tnil))). 
+Notation zeroH := (apply Zero Tnil).
+Notation succH t := (apply Succ (Tcons t Tnil)).
 Fixpoint termOfNat n :=
   match n with 
-    0 => zeroNN
-  | S p => succNN (termOfNat p)
+    0 => zeroH
+  | S p => succH (termOfNat p)
   end.
 (* end snippet instantiations *)
 
+Section Examples.
+
 (* begin snippet v1Plus01 *)
-Example t1: Term LNN := (plusNN (var 1) zeroNN). 
+Let t1: Term LNN := (plusH (var 1) zeroH). 
 (* end snippet v1Plus01 *)
 
 
-(** forall v0 v1, v0 < v1 -> v0 < v1 + v0 *)
+(** forall v0, v0 = 0 \/ exists v1,  v0 = S v1 *)
 (* begin snippet f1Example *)
-Example f1 : Formula LNN :=
-  forallNN 0 
-    (forallNN 1 
-       (impNN 
-          (ltNN (var 0) (var  1))
-          (ltNN (var 0) (plusNN (var 1) (var 0))))).  
+Let f1 : Formula LNN :=
+  forallH 0 
+    (orH (equal (var 0) zeroH)
+          (existH 1 (equal (var 0) (succH (var 1))))).
 (* end snippet f1Example *)
 
 (* begin snippet f2Example *)
-Example f2 : Formula LNN :=
-  forallNN 0 (existNN 1 (ltNN (var 0) (var 1))).
+Let f2 : Formula LNN :=
+   (existH 2 (andH (ltH zeroH (var 2))
+                 (equal (termOfNat 4) (plusH (var 2) (var 2))))).
+
+Let f3 := (orH (equal (var 0) zeroH)
+             (existH 1 (equal (var 0) (succH (var 1))))).
+
+Let f4 := (iffH (equal (var 0) (plusH (var 1) (var 1)))
+                (equal (var 0) (timesH (var 1) (termOfNat 2)))).
 (* end snippet f2Example *)
+
+(* begin snippet depthCompute *)
+Compute (depth _ f1, depth _ f2).
+(* end snippet depthCompute *)
+
+(* begin snippet FormulaRect *)
+About Formula_rect.
+(* end snippet FormulaRect *)
 
 (** depth-order vs structural order *)
 (* begin snippet ltDepth1:: no-out *)
-Goal lt_depth _ 
-  (existNN 1 (ltNN (plusNN (termOfNat 42) (var 3)) (var 1))) f2.
+Goal lt_depth _ f1  f2.
 Proof. red; cbn; auto with arith. Qed. 
 (* end snippet ltDepth1 *)
+
+(* begin snippet freeVarExamples *)
+Compute  freeVarFormula _ f3.
+
+Compute ListExt.no_dup _ Nat.eq_dec (freeVarFormula _ f3).
+
+Compute close _ f3.
+
+Compute freeVarFormula _ f3.
+
+Compute freeVarFormula _ (close _ f4).
+
+Compute substituteFormula LNN f4 0 (termOfNat 0).
+(* end snippet freeVarExamples *)
+
+End Examples. 
 End InLNN.
 
+Section depth_rec_demo. 
+Variable L: Language.
+Variable P: Formula L -> Prop. 
+Variable a: Formula L. 
+Goal P a. 
+  eapply  Formula_depth_rec_rec with (depth L a); [| apply le_n].
+  (* begin snippet depthRecDemo:: unfold no-in *)
+ clear a; intros a Ha.
+  (* end snippet depthRecDemo *)
+Abort.
+Goal P a. 
+ (* begin snippet depthRecDemo2:: unfold no-in *)
+ apply Formula_depth_ind2.
+ (* end snippet depthRecDemo2 *)
+Abort. 
 
+
+
+
+End depth_rec_demo. 
 
 
 
